src/proof/iam_model/attach.v
@@ -1,5 +1,5 @@
 From New.proof Require Import prelude empty_ffi.
-From New.proof.iam_model Require Export inv.
+From New.proof.iam_model Require Export common.
 
 Section proof.
 Context `{hG: !heapGS Σ} `{!ffi_semantics _ _}.
@@ -22,6 +22,157 @@ Lemma wp_State__AttachIdentityPolicy
       "Hattachments" ∷ own_iam_attachments_frag γ resource 1 (<[identity := n]> attachments) ∗
       "%Hn_positive" ∷ ⌜ (1 ≤ n)%nat ⌝
   }}}.
-Proof. Admitted.
+Proof.
+  iIntros (Φ) "(#Hiam & Hidentity & Hpolicy & Hattachments & %Hresource_eq) HΦ".
+  iDestruct "Hiam" as (mu_l) "[#Hmu #Hiam_inv]".
+  wp_method_call. rewrite /iammodel.State__AttachIdentityPolicyⁱᵐᵖˡ. wp_call.
+  wp_apply wp_with_defer as "%defer Hdefer". simpl subst. wp_auto.
+  wp_apply wp_Mutex__Lock;
+    [iFrame "#"; iEval (rewrite is_pkg_init_unfold /=);
+     iSplit; [iModIntro; iEval (rewrite !is_pkg_init_unfold /=); done|done]|].
+  iIntros "[Hown_Mutex H]". iNamedPrefix "H" "Hinv_". wp_auto.
+  iDestruct (own_identities_auth_frag_lookup with
+    "Hinv_Hown_identities_auth Hidentity") as %Hidentity_lookup.
+  iDestruct (own_policies_auth_frag_lookup with
+    "Hinv_Hown_policies_auth Hpolicy") as %Hpolicy_lookup.
+  iDestruct (big_sepM2_dom with "Hinv_Hown_phys_identities_inner") as %Hidentity_maps_dom.
+  assert (is_Some (phys_identities !! identity)) as [policy_ids_l Hphys_identity_lookup].
+  { apply elem_of_dom. rewrite Hidentity_maps_dom.
+    apply elem_of_dom. eexists. exact Hidentity_lookup. }
+  rewrite exception_do_unseal /exception_do_def.
+  wp_apply (wp_map_lookup2 iammodel.IdentityID
+    (go.MapType iammodel.PolicyID (go.StructType [])) with
+    "[$Hinv_Hown_phys_identities]") as "Hinv_Hown_phys_identities".
+  rewrite Hphys_identity_lookup /=.
+  wp_auto.
+  wp_apply (wp_map_lookup2 iammodel.PolicyID iammodel.IdentityPolicy
+    with "[$Hinv_Hown_phys_policies]") as "Hinv_Hown_phys_policies".
+  rewrite Hpolicy_lookup /=. wp_auto.
+  iDestruct (big_sepM2_delete _ phys_identities abs_identities
+    identity policy_ids_l policy_ids Hphys_identity_lookup Hidentity_lookup
+    with "Hinv_Hown_phys_identities_inner")
+    as "[Hown_policy_ids Hinv_Hown_phys_identities_inner]".
+  wp_apply (wp_map_lookup2 iammodel.PolicyID (go.StructType []) with
+    "[$Hown_policy_ids]") as "Hown_policy_ids".
+  destruct (policy_ids !! policy_id) as [[]|] eqn:Hattached.
+  - wp_auto.
+    assert (<[policy_id:=tt]> policy_ids = policy_ids) as Hpolicy_ids_same.
+    { apply insert_id. done. }
+    assert (<[identity:=<[policy_id:=tt]> policy_ids]> abs_identities =
+      abs_identities) as Hidentities_same.
+    { rewrite Hpolicy_ids_same. apply insert_id. done. }
+    iApply fupd_wp.
+    iMod (attach_identity_policy_vs
+      (γ:=γ.(γ_resource_access))
+      (identities:=abs_identities)
+      (identities':=abs_identities)
+      (policies:=phys_policies)
+      (observed_resources:=observed_resources)
+      (identity:=identity)
+      (policy_ids:=policy_ids)
+      (policy_id:=policy_id)
+      (policy:=policy)
+      (resource:=resource)
+      (attachments:=attachments)
+      with "Hinv_Hown_attachments_auth Hattachments")
+      as (n) "(Hinv_Hown_attachments_auth & Hattachments & %Hn_positive)".
+    { exact Hpolicy_lookup. }
+    { symmetry. exact Hresource_eq. }
+    { exact Hidentity_lookup. }
+    { symmetry. exact Hidentities_same. }
+    iModIntro.
+    iAssert (([∗ map] policy_ids_l'; policy_ids' ∈
+      phys_identities; abs_identities, policy_ids_l' ↦$ policy_ids')%I)
+      with "[Hown_policy_ids Hinv_Hown_phys_identities_inner]"
+      as "Hinv_Hown_phys_identities_inner".
+    { rewrite (big_sepM2_delete _ phys_identities abs_identities
+        identity policy_ids_l policy_ids Hphys_identity_lookup Hidentity_lookup).
+      iFrame. }
+    iCombineNamed "Hinv_*" as "H".
+    rewrite return_val_unseal /return_val_def. wp_auto.
+    wp_apply (wp_Mutex__Unlock _ (iam_inv γ l) with "[$Hown_Mutex H]").
+    { iNamed "H". iFrame. iFrame "#%".
+      iEval (rewrite is_pkg_init_unfold /=).
+      iSplit; [iModIntro; iEval (rewrite !is_pkg_init_unfold /=); done|done]. }
+    iApply ("HΦ" $! n). rewrite Hpolicy_ids_same. iFrame. done.
+  - wp_auto.
+    wp_apply (wp_map_insert iammodel.PolicyID with "[$Hown_policy_ids]").
+    iIntros "Hown_policy_ids". wp_auto.
+    iApply fupd_wp.
+    iMod (own_identity_update_vs
+      (γ:=γ.(γ_identities))
+      (identities:=abs_identities)
+      (identity:=identity)
+      (policy_ids:=policy_ids)
+      (policy_ids':=<[policy_id:=tt]> policy_ids)
+      with "Hinv_Hown_identities_auth Hidentity")
+      as "[Hinv_Hown_identities_auth Hidentity]".
+    iMod (attach_identity_policy_vs
+      (γ:=γ.(γ_resource_access))
+      (identities:=abs_identities)
+      (identities':=<[identity:=<[policy_id:=tt]> policy_ids]> abs_identities)
+      (policies:=phys_policies)
+      (observed_resources:=observed_resources)
+      (identity:=identity)
+      (policy_ids:=policy_ids)
+      (policy_id:=policy_id)
+      (policy:=policy)
+      (resource:=resource)
+      (attachments:=attachments)
+      with "Hinv_Hown_attachments_auth Hattachments")
+      as (n) "(Hinv_Hown_attachments_auth & Hattachments & %Hn_positive)".
+    { exact Hpolicy_lookup. }
+    { symmetry. exact Hresource_eq. }
+    { exact Hidentity_lookup. }
+    { done. }
+    iModIntro.
+    assert ((<[identity:=<[policy_id:=tt]> policy_ids]> abs_identities) !!
+      identity = Some (<[policy_id:=tt]> policy_ids)) as Hidentity_lookup_update.
+    { rewrite lookup_insert_eq. done. }
+    iAssert (([∗ map] policy_ids_l'; policy_ids' ∈
+      phys_identities; <[identity:=<[policy_id:=tt]> policy_ids]> abs_identities,
+      policy_ids_l' ↦$ policy_ids')%I)
+      with "[Hown_policy_ids Hinv_Hown_phys_identities_inner]"
+      as "Hinv_Hown_phys_identities_inner".
+    { rewrite (big_sepM2_delete _ phys_identities
+        (<[identity:=<[policy_id:=tt]> policy_ids]> abs_identities)
+        identity policy_ids_l (<[policy_id:=tt]> policy_ids)
+        Hphys_identity_lookup Hidentity_lookup_update).
+      rewrite delete_insert_eq. iFrame. }
+    iCombineNamed "Hinv_*" as "H".
+    rewrite return_val_unseal /return_val_def. wp_auto.
+    wp_apply (wp_Mutex__Unlock _ (iam_inv γ l) with "[$Hown_Mutex H]").
+    { iNamed "H". iFrame. iFrame "#".
+      iSplit.
+      - iEval (rewrite is_pkg_init_unfold /=).
+        iSplit; [iModIntro; iEval (rewrite !is_pkg_init_unfold /=); done|done].
+      - iNext. iSplit.
+        + iPureIntro.
+          intros identity' policy_ids' policy_id' Hidentity' Hattached'.
+          destruct (decide (identity' = identity)) as [->|Hidentity_ne].
+          * rewrite lookup_insert_eq in Hidentity'. inversion Hidentity'. subst policy_ids'.
+            destruct (decide (policy_id' = policy_id)) as [->|Hpolicy_ne].
+            -- exists policy. done.
+            -- assert (policy_id ≠ policy_id') as Hpolicy_ne' by congruence.
+               replace ((<[policy_id:=tt]> policy_ids) !! policy_id')
+                 with (policy_ids !! policy_id') in Hattached'.
+               2:{ symmetry. apply lookup_insert_ne. exact Hpolicy_ne'. }
+               destruct (Hinv_Hattached_policy_exists
+                 identity policy_ids policy_id' Hidentity_lookup Hattached')
+                 as [policy' Hpolicy'].
+               exists policy'. done.
+          * assert (identity ≠ identity') as Hidentity_ne' by congruence.
+            replace ((<[identity:=<[policy_id:=tt]> policy_ids]> abs_identities) !! identity')
+              with (abs_identities !! identity') in Hidentity'.
+            2:{ symmetry. apply lookup_insert_ne. exact Hidentity_ne'. }
+            destruct (Hinv_Hattached_policy_exists
+              identity' policy_ids' policy_id' Hidentity' Hattached')
+              as [policy' Hpolicy'].
+            exists policy'. done.
+        + iPureIntro. exact Hinv_Hexisting_policy_used. }
+    iApply ("HΦ" $! n). iFrame. done.
+Unshelve.
+  all: unfold iammodel.IdentityID.t, iammodel.PolicyID.t; apply _.
+Qed.
 
 End proof.
